\documentclass{article}
\usepackage[fleqn]{mathtools}
\usepackage{amsfonts} 

\begin{document}
\title{Math Shit}
\boldmath

\section{Constants}

\begin{equation}
\lim_{x\to\pm\infty}(1+\frac{1}{x})^x=e\approx2.7182
\end{equation}

\section{Limits}

Definition of limit:
\begin{equation}
\lim_{x\to{x_0}}f(x) = l \textnormal{ if } \forall\varepsilon<0\exists I(x_0): |f(x) - l| < \varepsilon, \forall x \in I(x_0), x\neq x_0
\end{equation}

A vertical asymptote of a function happens in $x = c$ if:
\begin{equation}
\lim_{x\to{c^\pm}} f(x) = \pm\infty
\end{equation}

A horizontal asymptote of a function happens in $y = c$ if:
\begin{equation}
\lim_{x\to{\pm\infty}} f(x) = \pm c
\end{equation}

An oblique asymptote of a function happens if:
\begin{equation}
\lim_{x\to{\pm\infty}} \frac{f(x)}{x} = m
\end{equation}
with $m \neq 0$.
to find $q$: 
\begin{equation}
\lim_{x\to{\pm\infty}} [f(x) - mx] = q
\end{equation}

Addition of limits
\begin{equation}
\lim_{x\to{x_0}} [f(x) + g(x)] = \lim_{x\to{x_0}} f(x) + \lim_{x\to{x_0}} g(x)
\end{equation}

Product of limits
\begin{equation}
\lim_{x\to{x_0}} [f(x) \cdot g(x)] = \lim_{x\to{x_0}} f(x) \cdot \lim_{x\to{x_0}} g(x)
\end{equation}

Division of limits
\begin{equation}
\lim_{x\to{x_0}} [\frac{f(x)}{g(x)}] = \frac{\lim_{x\to{x_0}} f(x)}{\lim_{x\to{x_0}} g(x)}
\end{equation}

Power
\begin{equation}
\lim_{x\to{x_0}} f(x) = l \in \mathbb{R} \Rightarrow \lim_{x\to{x_0}} [f(x)]^n = l^n, \forall n\in \mathbb{N} - \{0\}
\end{equation}

Indeterminate forms:
\begin{equation}
+\infty - \infty, \infty \cdot 0, \frac{\infty}{\infty}, \frac{0}{0}, 1^{\infty}, 0^0, \infty^0
\end{equation}

Common limits:
\begin{equation}
\lim_{x\to{0}} \frac{\sin{x}}{x} = 1
\end{equation}
\begin{equation}
\lim_{x\to{0}} \frac{1-\cos{x}}{x} = 0
\end{equation}
\begin{equation}
\lim_{x\to{0}} \frac{1-\cos{x}}{x^2} = \frac{1}{2}
\end{equation}
\begin{equation}
\lim_{x\to\pm\infty}1+\frac{1}{x}^x=e
\end{equation}
\begin{equation}
\lim_{x\to{0}}\frac{\ln{(1+x)}}{x}=1
\end{equation}
\begin{equation}
\lim_{x\to{0}}\frac{e^x-1}{x}=1
\end{equation}
\begin{equation}
\lim_{x\to{0}}\frac{\log_a{(1+x)}}{x}=\log_a{e}
\end{equation}
\begin{equation}
\lim_{x\to{0}}\frac{a^x-1}{x}=\ln{a}
\end{equation}
\begin{equation}
\lim_{x\to{0}}\frac{(1+x)^k-1}{x}=k
\end{equation}

\section{Derivatives}

Definition of derivative:
\begin{equation}
D[f(x)] = f'(x) = \lim_{h\to0}(\frac{f(x)-f(x+h)}{h})
\end{equation}

\section{Integrals}

\begin{equation}
\int_{a}^{b} f(x) dx = [F(x)]_{a}^{b} = F(b) - F(a)
\end{equation}

\end{document}